theories/L6_PCPS/eval.v
@@ -412,58 +412,67 @@ Section EVAL.
     inv H8; eauto.
   Qed.
 
+  Lemma bstep_cost_deterministic e rho v1 v2 c1 c2 :
+    bstep_cost rho e v1 c1 ->
+    bstep_cost rho e v2 c2 ->
+    v1 = v2 /\ c1 = c2.
+  Proof.
+    intros Heval1 Heval2.
+    revert v2 c2 Heval2; induction Heval1; intros v2 c2 Heval2;
+      inv Heval2; repeat subst_exp; eauto;
+        try now edestruct IHHeval1 as [Heq1 Heq2]; eauto.
+    + eapply find_tag_nth_deterministic in H7; [| clear H7; eauto ]; inv H7.
+      eapply IHHeval1 in H10. inv H10. split; congruence.
+    + eapply IHHeval1_1 in H15. inv H15.
+      eapply IHHeval1_2 in H16. inv H16.
+      split; congruence.
+  Qed.
 
-  (** Big step semantics with cost counting as fuel. Can raise out-of-time exception.
-      Needed to prove divergence preservation *)
+
+  (** Big step semantics with two notions of resource:
+      - an input one (fuel)
+      - an output one (trace)
+      Will raise OOT (out-of-time exception) if fuel is not enough,
+      the lets us prove divergence preservation *)
 
   Inductive res {A} : Type :=
   | OOT
   | Res : A -> res.
 
-  Definition cost (e : exp) : nat :=
-    match e with
-    | Econstr x t ys e => 1 (* + length ys *)
-    | Eproj x t n y e => 1
-    | Ecase y cl => 1
-    | Eapp f t ys => 1 (* + length ys *)
-    | Eletapp x f t ys e => 1 (* + length ys *)
-    | Efun B e => 1 (* + PS.cardinal (fundefs_fv B) *)
-    | Eprim x f ys e => 1 (* + length ys *)
-    | Ehalt x => 1
-    end.
   
-  Context {steps: Type} {Hr : @resource_exp steps}.
+  Context {fuel: Type} {Hf : @resource_exp fuel} {trace: Type} {Ht : @resource_exp trace}.
+  Context (Hro : @resource_ones fin fuel (@HRes _ Hf)).
 
   Open Scope alg_scope.
-
-  Inductive bstep :  env -> exp -> @res val -> steps -> Prop :=
+  
+  Inductive bstep :  env -> exp -> fuel -> @res val -> trace -> Prop :=
   | BStept_constr :
       forall (x : var) (t : ctor_tag) (ys :list var) (e : exp)
-             (rho rho' : env) (vs : list val) (v : res) (cin : steps),
+             (rho rho' : env) (vs : list val) (v : res) (cin : fuel) (cout : trace),
         get_list ys rho = Some vs ->
         M.set x (Vconstr t vs) rho = rho' ->
-        bstep_fuel rho' e v cin ->
-        bstep rho (Econstr x t ys e) v cin
+        bstep_fuel rho' e cin v cout ->
+        bstep rho (Econstr x t ys e) cin v cout
   | BStept_proj :
       forall (t : ctor_tag) (vs : list val)
              (rho : env) (x : var) (n : N) (y : var)
-             (e : exp) (v : val) (v' : res) (cin : steps),
+             (e : exp) (v : val) (v' : res) (cin : fuel) (cout : trace),
         M.get y rho = Some (Vconstr t vs) ->
         nthN vs n = Some v ->
-        bstep_fuel (M.set x v rho) e v' cin ->
-        bstep rho (Eproj x t n y e) v' cin
+        bstep_fuel (M.set x v rho) e cin v' cout ->
+        bstep rho (Eproj x t n y e) cin v' cout
   | BStept_case :
       forall (y : var) (v : res) (e : exp) (t : ctor_tag) (cl : list (ctor_tag * exp))
-             (vl : list val) (rho : env) (cin : steps) (n : nat),
+             (vl : list val) (rho : env) (cin : fuel) (n : nat) (cout : trace),
         M.get y rho = Some (Vconstr t vl) ->
         caseConsistent cenv cl t ->
         find_tag_nth cl t e n ->
-        bstep_fuel rho e v cin ->
-        bstep rho (Ecase y cl) v cin
+        bstep_fuel rho e cin v cout ->
+        bstep rho (Ecase y cl) cin v cout
   | BStept_app :
       forall (rho' : env) (fl : fundefs) (f' : var) (vs : list val)
              (xs : list var) (e : exp) (rho'' rho : env) (f : var)
-             (t : ctor_tag) (ys : list var) (v : res) (cin : steps),
+             (t : ctor_tag) (ys : list var) (v : res) (cin : fuel) (cout : trace),
         M.get f rho = Some (Vfun rho' fl f') ->
         get_list ys rho = Some vs ->
         (* The number of instructions generated here should be
@@ -471,37 +480,38 @@ Section EVAL.
          * jump to a label *)
         find_def f' fl = Some (t,xs,e) ->
         set_lists xs vs (def_funs fl fl rho' rho') = Some rho'' ->
-        bstep_fuel rho'' e v cin ->
-        bstep rho (Eapp f t ys) v cin
+        bstep_fuel rho'' e cin v cout ->
+        bstep rho (Eapp f t ys) cin v cout
   | BStept_letapp :
       forall (rho' : env) (fl : fundefs) (f' : var) (vs : list val)
              (xs : list var) (e_body e : exp) (rho'' rho : env) (x f : var)
-             (t : ctor_tag) (ys : list var) (v : val) (v' : res) (cin1 cin2 : steps),
+             (t : ctor_tag) (ys : list var) (v : val) (v' : res)
+             (cin1 cin2 : fuel) (cout1 cout2 : trace),
         (* evaluate application *)
         M.get f rho = Some (Vfun rho' fl f') ->
         get_list ys rho = Some vs ->
         find_def f' fl = Some (t,xs,e_body) ->
         set_lists xs vs (def_funs fl fl rho' rho') = Some rho'' ->
-        bstep_fuel rho'' e_body (Res v) cin1 -> (* body evaluates to v *)
+        bstep_fuel rho'' e_body cin1 (Res v) cout1 -> (* body evaluates to v *)
         (* evaluate let continuation *)
-        bstep_fuel (M.set x v rho) e v' cin2 ->
-        bstep rho (Eletapp x f t ys e) v' (cin1 <+> cin2)
+        bstep_fuel (M.set x v rho) e cin2 v' cout2 ->
+        bstep rho (Eletapp x f t ys e) (cin1 <+> cin2) v' (cout1 <+> cout2)
   | BStept_letapp_oot :
       forall (rho' : env) (fl : fundefs) (f' : var) (vs : list val)
              (xs : list var) (e_body e : exp) (rho'' rho : env) (x f : var)
-             (t : ctor_tag) (ys : list var) (cin : steps),
+             (t : ctor_tag) (ys : list var) (cin : fuel) (cout : trace),
         M.get f rho = Some (Vfun rho' fl f') ->
         get_list ys rho = Some vs ->
         find_def f' fl = Some (t,xs,e_body) ->
         set_lists xs vs (def_funs fl fl rho' rho') = Some rho'' ->
-        bstep_fuel rho'' e_body OOT cin -> (* body times out*)
-        bstep rho (Eletapp x f t ys e) OOT cin
+        bstep_fuel rho'' e_body cin OOT cout -> (* body times out*)
+        bstep rho (Eletapp x f t ys e) cin OOT cout
   | BStept_fun :
-      forall (rho : env) (B : fundefs) (e : exp) (v : res) (cin : steps),
-        bstep_fuel (def_funs B B rho rho) e v cin ->
+      forall (rho : env) (B : fundefs) (e : exp) (v : res) (cin : fuel) (cout : trace),
+        bstep_fuel (def_funs B B rho rho) e cin v cout ->
         (* The definition of a function incur cost proportional to the number of FVs
         (to make the bound of the current cc independent of the term) *)
-        bstep rho (Efun B e) v cin
+        bstep rho (Efun B e) cin v cout
   (* | BStept_prim :
       forall (vs : list val) (rho' rho : env) (x : var) (f : prim)
         (f' : list val -> option val) (ys : list var) (e : exp)
@@ -515,352 +525,460 @@ Section EVAL.
   | BStept_halt :
       forall x v rho,
         M.get x rho = Some v ->
-        bstep rho (Ehalt x) (Res v) <0>
-  with bstep_fuel :  env -> exp -> @res val -> steps -> Prop :=
-  | BStepf_OOT : (* not enought time units to take astep *)
-      forall rho (e : exp) (c : steps),
-        (c <<_{ e } <1> e) -> (* not enough steps *)
-        bstep_fuel rho e OOT c
+        bstep rho (Ehalt x) <0> (Res v) <0>
+  with bstep_fuel :  env -> exp -> fuel -> @res val -> trace -> Prop :=
+  | BStepf_OOT : (* not enought time units to take a step *)
+      forall rho (e : exp) (c : fuel),
+        (c << <1> e) -> (* not enough fuel *)
+        bstep_fuel rho e c OOT <0>
   | BStepf_run : (* take a step *)
-      forall rho e r (c : steps),
-        bstep rho e r c ->
-        bstep_fuel rho e r (c <+> (<1> e)).
+      forall rho e r (cin : fuel) (cout : trace),
+        bstep rho e cin r cout ->
+        bstep_fuel rho e (cin <+> (<1> e)) r (cout <+> (<1> e)).
 
   Scheme bstep_ind' := Minimality for bstep Sort Prop
     with bstep_fuel_ind' := Minimality for bstep_fuel Sort Prop.
   
   Definition not_stuck (rho : env) (e : exp) :=
-    (exists c v, bstep_fuel rho e (Res v) c) \/
-    (forall c, bstep_fuel rho e OOT c).
+    (exists cin v cout, bstep_fuel rho e cin (Res v) cout) \/
+    (forall cin, exists cout, bstep_fuel rho e cin OOT cout).
 
   Ltac destruct_bstep :=
     match goal with
     | [ H : bstep _ _ _ _ |- _ ] => inv H
     end.
 
-  Lemma cost_gt_0 e : 
-    (0 < cost e)%nat.
-  Proof.  
-    destruct e; simpl; omega. 
-  Qed.
 
   (** * Lemmas about bstep_fuel *)
-  Lemma step_deterministic_aux rho e r v c r' v' c' :
-    bstep rho e r c ->
-    bstep rho e r' c' ->
+  Lemma step_deterministic_aux rho e r v cin cin' r' v' cout cout' :
+    bstep rho e cin r cout ->
+    bstep rho e cin' r' cout' ->
     r = Res v -> r' = Res v' ->
-    v = v' /\ c = c'.
+    v = v' /\ cin = cin' /\ cout = cout'.
   Proof.
-    set (P := fun rho e r c =>
-                forall v r' v' c',
-                  bstep rho e r' c' ->
+    set (P := fun rho e cin r cout =>
+                forall v cin' r' v' cout',
+                  bstep rho e cin' r' cout' ->
                   r = Res v -> r' = Res v' ->
-                  v = v' /\ c = c').
-    set (P0 := fun rho e r c =>
-                 forall v r' v' c',
-                   bstep_fuel rho e r' c' ->
+                  v = v' /\ cin = cin' /\ cout = cout').
+    set (P0 := fun rho e cin r cout =>
+                 forall v cin' r' v' cout',
+                   bstep_fuel rho e cin' r' cout' ->
                    r = Res v -> r' = Res v' ->
-                   v = v' /\ c = c').
+                   v = v' /\ cin = cin' /\ cout = cout').
     intros Hstep.
-    revert v r' v' c'.
+    revert v cin' r' v' cout'.
     induction Hstep using bstep_ind' with (P := P) (P0 := P0); unfold P, P0 in *;
-      intros v1 r2 v2 c2 Hstep2 Heq1 Heq2; subst;
+      intros v1 r2 v2 cin2' cout2' Hstep2 Heq1 Heq2; subst;
         try now (inv Hstep2; repeat subst_exp; eapply IHHstep; eauto).
     - inv Hstep2. repeat subst_exp.
       eapply find_tag_nth_deterministic in H1; [| eapply H8 ]. inv H1.
       eapply IHHstep; eauto.
-    - inv Hstep2. repeat subst_exp. eapply IHHstep in H17; eauto. inv H17.
-      eapply IHHstep0 in H18; eauto. inv H18. eauto.
+    - inv Hstep2. repeat subst_exp. eapply IHHstep in H18; eauto. destructAll.
+      eapply IHHstep0 in H19; eauto. destructAll. eauto.
     - inv Hstep2. inv Heq1. repeat subst_exp. eauto.
     - inv Heq1.
-    - inv Hstep2. eapply IHHstep in H; eauto. inv H.
-      split; eauto.
+    - inv Hstep2. eapply IHHstep in H; eauto.  destructAll. eauto.
   Qed.
 
-  Lemma bstep_fuel_deterministic rho e v c v' c' :
-    bstep_fuel rho e (Res v) c ->
-    bstep_fuel rho e (Res v') c' ->
-    v = v' /\ c = c'.
+  Lemma bstep_fuel_deterministic rho e v cin cin' v' cout cout' :
+    bstep_fuel rho e cin (Res v) cout ->
+    bstep_fuel rho e cin' (Res v') cout' ->
+    v = v' /\ cin = cin' /\ cout = cout'.
   Proof.
     intros H1 H2; inv H1; inv H2; eauto.
     eapply step_deterministic_aux in H0; [ | eapply H | reflexivity | reflexivity ].
-    inv H0. split; eauto.
+    destructAll; eauto.
   Qed.
 
-  Lemma bstep_deterministic rho e v c v' c' :
-    bstep rho e (Res v) c ->
-    bstep rho e (Res v') c' ->
-    v = v' /\ c = c'.
+  Lemma bstep_deterministic rho e v cin cin' v' cout cout' :
+    bstep rho e cin (Res v) cout ->
+    bstep rho e cin' (Res v') cout' ->
+    v = v' /\ cin = cin' /\ cout = cout'.
   Proof.
     intros H1 H2. eapply step_deterministic_aux; eauto.
   Qed.
 
-  Lemma bstep_lt_OOT_aux rho e r c (v : val) c' i:
-    bstep rho e r c ->
+        
+  Lemma bstep_lt_OOT_aux rho e r cin (v : val) cout cin':
+    bstep rho e cin r cout ->
     r = Res v ->
-    (c' <<_{ i } c) -> (* the resource is smaller in any dimention *)
-    bstep rho e OOT c'.
+    cin' << cin ->
+    exists cout' c, bstep rho e cin' OOT cout' /\ cout = (c <+> cout').
   Proof.
-    set (P := fun rho e r c =>
-                forall i (v : val) c',
-  		  r = Res v -> c' <<_{ i } c ->
-		  bstep rho e OOT c').
-    set (P0 := fun rho e r c =>
-                 forall i (v : val) c',
-  		   r = Res v -> c' <<_{ i } c ->
-		   bstep_fuel rho e OOT c').
-    intros Hstep. revert i v c'.
+    set (P := fun rho e cin r cout =>
+                forall (v : val) cin',
+  		  r = Res v -> cin' << cin ->
+		  exists cout' c, bstep rho e cin' OOT cout' /\ cout = (c <+> cout')).
+    set (P0 := fun rho e cin r cout =>
+                 forall (v : val) cin',
+  		   r = Res v -> cin' << cin ->
+		   exists cout' c, bstep_fuel rho e cin' OOT cout' /\ cout = (c <+> cout')).
+    intros Hstep. revert v cin'.
     induction Hstep using bstep_ind' with (P := P) (P0 := P0); unfold P, P0 in *;
-      intros i v1 c' Heq Hlt; subst; try now (econstructor; eauto).
-    - edestruct (lt_all_dec_exp c' cin1).
-      + inv H5. eapply BStept_letapp_oot; eauto.
-      + inv H5. 
-        rewrite plus_comm. eapply BStept_letapp; eauto. eapply IHHstep0. reflexivity.
-        rewrite (plus_comm cin1) in Hlt. eapply plus_stable in Hlt. eassumption.
+      intros v1 cin' Heq Hlt; subst;
+    try (now edestruct IHHstep;
+         [reflexivity | eassumption | destructAll; do 2 eexists; split; eauto; econstructor; eauto ]).
+
+    - edestruct (lt_all_dec cin' cin1).
+      + edestruct IHHstep. reflexivity. eassumption. destructAll.
+        do 2 eexists. split. eapply BStept_letapp_oot; eauto. rewrite plus_assoc. rewrite (plus_comm x0).
+        rewrite <- plus_assoc. reflexivity.
+      + inv H5. rewrite (plus_comm cin1) in Hlt. eapply plus_stable in Hlt.
+        edestruct IHHstep0. reflexivity. eassumption. destructAll. 
+        do 2 eexists. split. rewrite plus_comm. 
+        eapply BStept_letapp; eauto.
+        rewrite <- !plus_assoc. rewrite (plus_comm cout1). reflexivity.
+    - inv Heq.
     - eapply lt_zero in Hlt. contradiction.
-    - edestruct (lt_dec_i c' (exp_to_fin e)).
-      + econstructor 1; eauto.
-      + inv H. econstructor 2. eapply IHHstep. reflexivity.
-        eapply plus_stable in Hlt. eassumption.
+    - inv Heq.
+    - edestruct (lt_all_dec cin' (one e)).
+      + subst. do 2 eexists. split. econstructor 1; eauto.
+        rewrite (plus_comm _ <0>). rewrite plus_zero. reflexivity.
+      + destructAll. eapply plus_stable in Hlt.
+        edestruct IHHstep. reflexivity. eassumption. destructAll.
+        do 2 eexists. split. econstructor 2. eassumption. rewrite plus_assoc. reflexivity.
   Qed.
 
-  Lemma bstep_lt_OOT rho e v c c' i :
-    bstep rho e (Res v) c ->
-    c' <<_{ i } c ->
-    bstep rho e OOT c'.
+  Lemma bstep_lt_OOT rho e v cin cout cin' :
+    bstep rho e cin (Res v) cout ->
+    cin' << cin ->
+    exists cout' c, bstep rho e cin' OOT cout' /\ cout = (c <+> cout').
   Proof.
-    intros; eapply bstep_lt_OOT_aux; eauto.
+    intros Hbstep Hlt. eapply bstep_lt_OOT_aux; eauto.
   Qed.
-
-  Lemma bstep_fuel_lt_OOT rho e v c c' i :
-    bstep_fuel rho e (Res v) c ->
-    c' <<_{ i } c ->
-    bstep_fuel rho e OOT c'.
+  
+  Lemma bstep_fuel_lt_OOT rho e v cin cout cin' :
+    bstep_fuel rho e cin (Res v) cout ->
+    cin' << cin ->
+    exists cout' c, bstep_fuel rho e cin' OOT cout' /\ cout = (c <+> cout').
   Proof.
     intros H1 Hlt; inv H1.
-    edestruct (lt_dec_i c' (exp_to_fin e)).
-    + econstructor 1; eauto.
-    + inv H0. econstructor 2. eapply bstep_lt_OOT. eassumption.
-      eapply plus_stable in Hlt. eassumption.
-  Qed.        
+    edestruct (lt_all_dec cin' (one e)).
+      + subst. do 2 eexists. split. econstructor 1; eauto.
+        rewrite (plus_comm _ <0>). rewrite plus_zero. reflexivity.
+      + destructAll. eapply plus_stable in Hlt.
+        edestruct bstep_lt_OOT. eassumption. eassumption. destructAll.
+        do 2 eexists. split. econstructor 2. eassumption. rewrite plus_assoc. reflexivity.
+  Qed.
 
-  Lemma bstep_OOT_determistic_aux rho e (r r' : @res val) c1 c2 c :
-    bstep rho e r c ->
-    r = OOT ->
-    c = (c1 <+> c2) ->
-    bstep rho e r' c1 -> r' = OOT.
+  
+  Lemma bstep_OOT_subtrace_aux rho e (r : @res val) v cin cout cin' cout' :
+    bstep rho e cin r cout ->
+    r = Res v ->
+    bstep rho e cin' OOT cout' ->
+    (exists c', cout = (c' <+> cout')).
   Proof.
-    set (P := fun rho e (r : @res val) c =>
-                forall r' c1 c2,
-                  r = OOT ->
-                  c = (c1 <+> c2) ->
-                  bstep rho e r' c1 -> r' = OOT).
-    set (P0 := fun rho e (r : @res val) c =>
-                 forall r' c1 c2,
-                   r = OOT ->
-                   c = (c1 <+> c2) ->
-                   bstep_fuel rho e r' c1 -> r' = OOT).
-    intros Hstep. revert r' c1 c2.
-    induction Hstep using bstep_ind' with (P := P) (P0 := P0); unfold P, P0 in *;
-      intros r' c1 c2 Heq Hleq Hs'; subst; try now (inv Hs'; repeat subst_exp; eauto).
+    set (P := fun rho e (cin : fuel) (r : @res val) cout =>
+                forall v cin' cout',
+                  r = Res v ->
+                  bstep rho e cin' OOT cout' ->
+                  (exists c', cout = (c' <+> cout'))).
+    set (P0 := fun rho e (cin : fuel) (r : @res val) cout =>
+                forall v cin' cout',
+                  r = Res v ->
+                  bstep_fuel rho e cin' OOT cout' ->
+                  (exists c', cout = (c' <+> cout'))).
+    intros Hstep. revert v cin' cout'.
+    induction Hstep using bstep_ind' with (P := P) (P0 := P0); unfold P, P0 in *;    
+    intros v1 cin' cout' Heq Hs'; try (now subst; inv Hs'; repeat subst_exp; eauto).
     - inv Hs'; repeat subst_exp. eapply find_tag_nth_deterministic in H8; [| clear H8; eauto ]. inv H8.
       eapply IHHstep; eauto.
     - inv Hs'; repeat subst_exp; eauto.
-      eapply bstep_fuel_deterministic in H17; [| clear H17; eauto ]; inv H17.
-      eapply IHHstep0; [| | eassumption ]; eauto. rewrite plus_assoc, !(plus_comm cin0) in Hleq.
-      eapply plus_inv in Hleq. subst. reflexivity.
-    - inv Hs'; repeat subst_exp; eauto. exfalso.
-      eapply IHHstep in H16; eauto. congruence. rewrite plus_assoc. reflexivity.
-    - inv Hs'; eauto. eapply plus_lt in H. rewrite plus_comm in H. eapply plus_lt in H.
-      eapply lt_antisym in H. contradiction. 
-    - inv Hs'; eauto. eapply IHHstep; [| | eassumption ]; eauto.
-      rewrite plus_assoc, !(plus_comm _ c2), <- plus_assoc in Hleq.
-      eapply plus_inv in Hleq. subst. reflexivity.
+      + eapply bstep_fuel_deterministic in H18; [| clear H18; eauto ]; destructAll.
+        edestruct IHHstep0; [| eassumption | ]; eauto. subst.
+        eexists.
+        rewrite <- (plus_assoc cout0). rewrite (plus_comm cout0) at 1.
+        rewrite plus_assoc at 1. reflexivity.
+      + edestruct IHHstep; [| eassumption | ]; eauto. subst.
+        eexists.
+        rewrite (plus_assoc x0). rewrite (plus_comm cout') at 1.
+        rewrite <- plus_assoc at 1. reflexivity.
+    - subst. inv Hs'; repeat subst_exp; eauto.
+      + eexists. rewrite (plus_comm _ <0>). rewrite plus_zero. reflexivity.
+      + eapply IHHstep in H; eauto. destructAll.
+        eexists.
+        rewrite plus_assoc at 1. reflexivity.
   Qed.
 
-  Lemma bstep_OOT_determistic rho e r' c1 c2 :
-    bstep rho e OOT (c1 <+> c2) ->
-    bstep rho e r' c1 -> r' = OOT.
+  Lemma bstep_OOT_subtrace rho e v cin cout cin' cout' :
+    bstep rho e cin (Res v) cout ->
+    bstep rho e cin' OOT cout' ->
+    (exists c', cout = (c' <+> cout')).
+  Proof.
+    intros Hs1 Hs2. eapply bstep_OOT_subtrace_aux. eassumption. reflexivity. eassumption.
+  Qed.
+
+  Lemma bstep_fuel_OOT_subtrace rho e v cin cout cin' cout' :
+    bstep_fuel rho e cin (Res v) cout ->
+    bstep_fuel rho e cin' OOT cout' ->
+    (exists c', cout = (c' <+> cout')).
+  Proof.
+    intros Hs1 Hs2. inv Hs1. inv Hs2.
+    + eexists. rewrite (plus_comm _ <0>). rewrite plus_zero. reflexivity.
+    + eapply bstep_OOT_subtrace in H; eauto. destructAll.
+      eexists.
+      rewrite plus_assoc at 1. reflexivity.
+  Qed.
+
+  
+  Lemma bstep_OOT_determistic_aux rho e (r r' : @res val) cin cout cin' cout' c :    
+    bstep rho e cin r cout ->
+    r = OOT ->
+    cin = (c <+> cin') ->
+    bstep rho e cin' r' cout' ->
+    r' = OOT /\ (exists c', cout = (c' <+> cout')).
+  Proof.
+    set (P := fun rho e cin (r : @res val) cout =>
+                forall r' cin' cout' c,
+                  r = OOT ->
+                  cin = (c <+> cin') ->
+                  bstep rho e cin' r' cout' ->
+                  r' = OOT /\ (exists c', cout = (c' <+> cout'))).
+    set (P0 := fun rho e cin (r : @res val) cout =>
+                 forall r' cin' cout' c,
+                   r = OOT ->
+                   cin = (c <+> cin') ->
+                   bstep_fuel rho e cin' r' cout' ->
+                   r' = OOT /\ (exists c', cout = (c' <+> cout'))).
+    intros Hstep. revert r' cin' cout' c.
+    induction Hstep using bstep_ind' with (P := P) (P0 := P0); unfold P, P0 in *;
+      intros r' cin' cout' c1 Heq Hleq Hs'; subst; try now (inv Hs'; repeat subst_exp; eauto).
+    - inv Hs'; repeat subst_exp. eapply find_tag_nth_deterministic in H8; [| clear H8; eauto ]. inv H8.
+      eapply IHHstep; eauto.
+    - inv Hs'; repeat subst_exp; eauto.
+      + eapply bstep_fuel_deterministic in H18; [| clear H18; eauto ]; destructAll.
+        rewrite !(plus_comm cin0), <- plus_assoc in Hleq.
+        eapply plus_inv in Hleq. subst.
+        edestruct IHHstep0; [| | eassumption | ]; eauto. destructAll. split; eauto. eexists. 
+        rewrite <- (plus_assoc cout0). rewrite (plus_comm cout0) at 1.
+        rewrite plus_assoc at 1. reflexivity.
+      + split. reflexivity.
+        eapply bstep_fuel_OOT_subtrace in H3; [| eassumption ]. destructAll.
+        eexists.
+        rewrite (plus_assoc x0). rewrite (plus_comm cout') at 1.
+        rewrite <- plus_assoc at 1. reflexivity.      
+    - inv Hs'; repeat subst_exp; eauto. exfalso.
+      eapply IHHstep in H17; eauto. inv H17. congruence.
+      rewrite (plus_comm cin1). rewrite <- plus_assoc. reflexivity.
+    - inv Hs'; eauto.
+      + split; eauto. eexists <0>. rewrite plus_zero. reflexivity.
+      + rewrite <- plus_assoc, plus_comm in H. eapply plus_lt in H.
+        eapply lt_antisym in H. contradiction. 
+    - inv Hs'; eauto.
+      + split; eauto. eexists. rewrite (plus_comm _ <0>). rewrite plus_zero. reflexivity.
+      + rewrite <- plus_assoc in Hleq. eapply plus_inv in Hleq. subst.
+        edestruct IHHstep. reflexivity. reflexivity. eassumption. destructAll.
+        split. reflexivity. eexists. rewrite plus_assoc. reflexivity.
+  Qed.
+
+  Lemma bstep_OOT_determistic rho e r' cin cout c cout' :
+    bstep rho e (c <+> cin) OOT cout ->
+    bstep rho e cin r' cout' ->
+    r' = OOT /\ (exists c', cout = (c' <+> cout')).
   Proof.
     intros; eapply bstep_OOT_determistic_aux; [ | reflexivity | | ]; eauto.
   Qed.
 
-  Lemma bstep_fuel_OOT_determistic rho e r' c1 c2 :
-    bstep_fuel rho e OOT (c1 <+> c2) ->
-    bstep_fuel rho e r' c1 -> r' = OOT.
+  Lemma bstep_fuel_OOT_determistic rho e r' cin cout c cout' :
+    bstep_fuel rho e (c <+> cin) OOT cout ->
+    bstep_fuel rho e cin r' cout' ->
+    r' = OOT /\ (exists c', cout = (c' <+> cout')).
   Proof.
-    intros Hs Hs'; inv Hs'; inv Hs; eauto.
-    - eapply plus_lt in H0. rewrite plus_comm in H0. eapply plus_lt in H0.
-      eapply lt_antisym in H0. contradiction. 
-    - rewrite plus_assoc, !(plus_comm _ c2), <- plus_assoc in H0.
-      eapply plus_inv in H0. subst.
-      eapply bstep_OOT_determistic; eauto.
+    intros Hs1 Hs2. inv Hs1.
+    - inv Hs2; eauto.
+      + split; eauto. eexists <0>. rewrite plus_zero. reflexivity.
+      + rewrite <- plus_assoc, plus_comm in H. eapply plus_lt in H.
+        eapply lt_antisym in H. contradiction. 
+    - inv Hs2; eauto.
+      + split; eauto. eexists. rewrite (plus_comm _ <0>). rewrite plus_zero. reflexivity.
+      + rewrite <- plus_assoc in H. eapply plus_inv in H. subst.
+        edestruct bstep_OOT_determistic_aux. eapply H2. reflexivity. reflexivity. eassumption.
+        destructAll.
+        split. reflexivity. eexists. rewrite plus_assoc. reflexivity.
   Qed.
 
-  Lemma bstep_gt_aux rho e r c (v : val) r' c' :
-    bstep rho e r c ->
-    r = Res v -> (forall i, c <<_{ i } c') ->
-    ~ bstep rho e r' c'.
+
+  
+  Lemma bstep_gt_aux rho e r cin (v : val) cout cin' r' cout' :
+    bstep rho e cin r cout ->
+    r = Res v -> cin << cin' ->
+    ~ bstep rho e cin' r' cout'.
   Proof.
-    set (P := fun rho e r c =>
-                forall (v : val) r' c',
-                  r = Res v -> (forall i, c <<_{ i } c') ->
-                  ~ bstep rho e r' c').
-    set (P0 := fun rho e r c =>
-                 forall (v : val) r' c',
-                   r = Res v -> (forall i, c <<_{ i } c') ->
-                   ~ bstep_fuel rho e r' c').
-    intros Hstep. revert v r' c'.
+    set (P := fun rho e cin r (cout : trace) =>
+                forall (v : val) r' cin' cout',
+                  r = Res v ->
+                  cin << cin' ->
+                  ~ bstep rho e cin' r' cout').
+    set (P0 := fun rho e cin r (cout : trace) =>
+                forall (v : val) r' cin' cout',
+                  r = Res v ->
+                  cin << cin' ->
+                  ~ bstep_fuel rho e cin' r' cout').
+    intros Hstep. revert v r' cin' cout'.
     induction Hstep using bstep_ind' with (P := P) (P0 := P0); unfold P, P0 in *;
-      intros v1 r' c' Heq Hlt Hstep'; subst; (try now (inv Hstep'; repeat subst_exp; eauto));
+      intros v1 r' cin' cout' Heq Hlt Hstep'; subst; (try now (inv Hstep'; repeat subst_exp; eauto));
         try now (inv Hstep'; repeat subst_exp; eauto; eapply IHHstep; eauto).
     - inv Hstep'; repeat subst_exp; eauto.
       eapply find_tag_nth_deterministic in H8; [| clear H8; eauto ]. inv H8.
       eapply IHHstep; eauto.
     - inv Hstep'; repeat subst_exp; eauto. 
-      + eapply bstep_fuel_deterministic in H17; [| clear H17; eauto ]; inv H17; subst.             
-        eapply IHHstep0; [| | eapply H18 ]. reflexivity.
-        intros i. specialize (Hlt i). rewrite !(plus_comm cin0) in Hlt. eapply plus_stable in Hlt. 
+      + eapply bstep_fuel_deterministic in H18; [| clear H18; eauto ]; destructAll.
+        eapply IHHstep0; [| | eapply H19 ]. reflexivity.
+        rewrite !(plus_comm cin0) in Hlt. eapply plus_stable in Hlt. 
         eassumption.
       + eapply IHHstep; [| | eassumption ]. reflexivity.
-        intros i. eapply plus_lt. eapply Hlt.
-    - inv Hstep'. eapply lt_antisym. eapply Hlt.
+        eapply plus_lt. eapply Hlt.
+    - inv Hstep'. eapply lt_antisym in Hlt. contradiction.
     - inv Hstep'.
-      + eapply lt_antisym. eapply lt_trans. eassumption.
-        eapply plus_lt. rewrite plus_comm. eapply Hlt. 
+      + rewrite plus_comm in Hlt. eapply plus_lt in Hlt.
+        eapply lt_trans in Hlt. specialize (Hlt H). eapply lt_antisym in Hlt. eassumption. 
       + eapply IHHstep; [| | eassumption ]. reflexivity.
-        intros i. specialize (Hlt i). eapply plus_stable in Hlt. eassumption.
-
-        Grab Existential Variables. exact (Ehalt xH). 
+        eapply plus_stable in Hlt. eassumption.
   Qed.
 
-  Lemma bstep_gt rho e r c v c' :
-    bstep rho e (Res v) c ->
-    (forall i, c <<_{ i } c') ->
-    ~ bstep rho e r c'.
+  Lemma bstep_gt rho e cin (v : val) cout cin' r cout' :
+    bstep rho e cin (Res v) cout ->
+    cin << cin' ->
+    ~ bstep rho e cin' r cout'.
   Proof.
     intros; eapply bstep_gt_aux; eauto.
   Qed.
-  
-  Lemma bstep_fuel_gt rho e r c v c' :
-    bstep_fuel rho e (Res v) c ->
-    (forall i, c <<_{ i } c') ->
-    ~ bstep_fuel rho e r c'.
+
+  Lemma bstep_fuel_gt rho e cin (v : val) cout cin' r cout' :
+    bstep_fuel rho e cin (Res v) cout ->
+    cin << cin' ->
+    ~ bstep_fuel rho e cin' r cout'.
   Proof.
     intros Hstep Hlt Hstep'. inv Hstep. inv Hstep'.
-    - eapply lt_antisym. eapply lt_trans. eassumption.
-        eapply plus_lt. rewrite plus_comm. eapply Hlt. 
-    - eapply bstep_gt; [ eassumption | | eassumption ].
-      intros i. specialize (Hlt i). eapply plus_stable in Hlt. eassumption.
+    - rewrite plus_comm in Hlt. eapply plus_lt in Hlt.
+      eapply lt_trans in Hlt. specialize (Hlt H0). eapply lt_antisym in Hlt. eassumption. 
+    - eapply bstep_gt; [| | eassumption ]. eassumption.
+      eapply plus_stable in Hlt. eassumption.
   Qed.
 
-  Lemma bstep_OOT_monotonic_aux rho e r (c c1 c2 : steps):
-    bstep rho e r c ->
+  Lemma bstep_OOT_monotonic_aux rho e r cin cout cin' c :
+    bstep rho e cin r cout ->
     r = OOT ->
-    c = (c1 <+> c2) ->
-    bstep rho e OOT c1.
+    cin = (c <+> cin') ->
+    exists cout' c, bstep rho e cin' OOT cout' /\ cout = (c <+> cout').
   Proof.
-    set (P := fun rho e (r : @res val) c =>
-                forall c1 c2,
+    set (P := fun rho e cin (r : @res val)  (cout : trace) =>
+                forall c cin',
                   r = OOT ->
-                  c = (c1 <+> c2) ->
-                  bstep rho e OOT c1).
-    set (P0 := fun rho e (r : @res val) c =>
-                 forall c1 c2,
+                  cin = (c <+> cin') ->
+                  exists cout' c, bstep rho e cin' OOT cout' /\ cout = (c <+> cout')).
+    set (P0 := fun rho e cin (r : @res val)  (cout : trace) =>
+                 forall c cin',
                    r = OOT ->
-                   c = (c1 <+> c2) ->
-                   bstep_fuel rho e OOT c1).
-    intros Hstep. revert c1 c2. 
+                   cin = (c <+> cin') ->
+                   exists cout' c, bstep_fuel rho e cin' OOT cout' /\ cout = (c <+> cout')).
+    intros Hstep. revert c cin'. 
     induction Hstep using bstep_ind' with (P := P) (P0 := P0); unfold P, P0 in *;
-    intros c1 c2 Heq Hleq; subst; try now (econstructor; eauto).
-    - edestruct (lt_all_dec_exp c1 cin1).
-      + inv H5. eapply BStept_letapp_oot; eauto.
-        eapply bstep_fuel_lt_OOT. eassumption. eassumption.
-      + inv H5. rewrite (plus_comm x0), plus_assoc in Hleq.
-        rewrite !(plus_comm cin1) in Hleq. eapply plus_inv in Hleq. subst.
-        rewrite plus_comm. eapply BStept_letapp; eauto.
-    - inv Heq.
-    - econstructor. eapply plus_lt. eassumption.
-    - edestruct (lt_dec_i c1 (exp_to_fin e)).
-      now econstructor; eauto. inv H.
-      rewrite plus_assoc, (plus_comm _ c2), <- plus_assoc in Hleq.
-      eapply plus_inv in Hleq. econstructor 2; eauto.
+      intros c' cin' Heq Hleq; subst;
+        try now (edestruct IHHstep; eauto; destructAll; do 2 eexists; split;
+                 [ econstructor; eauto | reflexivity ]).
+    - edestruct (lt_all_dec cin' cin1).
+      + edestruct bstep_fuel_lt_OOT. eassumption. eassumption. destructAll.
+        do 2 eexists. split. eapply BStept_letapp_oot; eauto.
+        rewrite plus_assoc. rewrite (plus_comm x0). rewrite <- plus_assoc. reflexivity.
+      + inv H5. rewrite <- plus_assoc, (plus_comm cin1) in Hleq.
+        eapply plus_inv in Hleq. subst.
+        edestruct IHHstep0. reflexivity. reflexivity. destructAll.
+        do 2 eexists. split. rewrite plus_comm. econstructor; eauto.
+        rewrite <- plus_assoc. rewrite (plus_comm _ x2). rewrite plus_assoc. reflexivity.
+    - congruence.
+    - do 2 eexists. split. econstructor 1. eapply plus_lt. rewrite plus_comm. eassumption.
+      rewrite plus_zero. reflexivity.
+    - edestruct (lt_all_dec cin' (one e)).
+      + do 2 eexists. split. 
+        now econstructor; eauto. rewrite (plus_comm _ <0>). rewrite plus_zero. reflexivity.
+      + destructAll. rewrite <- plus_assoc in Hleq. eapply plus_inv in Hleq. subst.
+        edestruct IHHstep. reflexivity. reflexivity. destructAll.
+        do 2 eexists. split. econstructor 2; eauto. rewrite plus_assoc. reflexivity.
   Qed.
 
-  Lemma bstep_OOT_monotonic rho e c1 c2 :
-    bstep rho e OOT (c1 <+> c2) ->
-    bstep rho e OOT c1.
+  Lemma bstep_OOT_monotonic rho e c1 c2 cout :
+    bstep rho e (c1 <+> c2) OOT cout ->
+    exists cout' c, bstep rho e c2 OOT cout' /\ cout = (c <+> cout').
   Proof.
     intros; eapply bstep_OOT_monotonic_aux; eauto.
   Qed.
-  
-  Lemma bstep_fuel_OOT_monotonic rho e c1 c2 :
-    bstep_fuel rho e OOT (c1 <+> c2) ->   
-    bstep_fuel rho e OOT c1.
-  Proof.
-    intros H1. inv H1.
-    - econstructor. eapply plus_lt. eassumption.
-    - edestruct (lt_dec_i c1 (exp_to_fin e)).
-      now econstructor; eauto. inv H0.
-      rewrite plus_assoc, (plus_comm _ c2), <- plus_assoc in H.
-      eapply plus_inv in H. econstructor 2. subst. eapply bstep_OOT_monotonic; eauto.
-  Qed. 
 
-  Lemma bstep_fuel_zero_OOT rho e :
-    bstep_fuel rho e OOT <0>.
+  Lemma bstep_fuel_OOT_monotonic rho e c1 c2 cout :
+    bstep_fuel rho e (c1 <+> c2) OOT cout ->
+    exists cout' c, bstep_fuel rho e c2 OOT cout' /\ cout = (c <+> cout').
   Proof.
-    econstructor. eapply zero_one_lt_i.
+    intros Hs; inv Hs.
+    - do 2 eexists. split. econstructor 1. eapply plus_lt. rewrite plus_comm. eassumption.
+      rewrite plus_zero. reflexivity.
+    - edestruct (lt_all_dec c2 (one e)).
+      + do 2 eexists. split. 
+        now econstructor; eauto. rewrite (plus_comm _ <0>). rewrite plus_zero. reflexivity.
+      + destructAll. rewrite <- plus_assoc in H. eapply plus_inv in H. subst.
+        edestruct bstep_OOT_monotonic. eassumption. destructAll.
+        do 2 eexists. split. econstructor 2; eauto. rewrite plus_assoc. reflexivity.
+  Qed.
+
+  
+  Lemma bstep_fuel_zero_OOT rho e :
+    bstep_fuel rho e <0> OOT <0>.
+  Proof.
+    econstructor. eapply zero_one_lt.
   Qed.
     
-  Lemma bstep_deterministic_res rho e r c r' :
-    bstep rho e r c ->
-    bstep rho e r' c ->
-    r = r'.
+  Lemma bstep_deterministic_res rho e cin r r' cout cout' :
+    bstep rho e cin r cout ->
+    bstep rho e cin r' cout' ->
+    r = r' /\ cout = cout'.
   Proof.
-    set (P := fun rho e r c =>
-                forall r',
-                  bstep rho e r' c ->
-                  r = r').
-    set (P0 := fun rho e r c =>
-                 forall r',
-                   bstep_fuel rho e r' c ->
-                   r = r').
+    set (P := fun rho e cin r cout =>
+                forall r' cout',
+                  bstep rho e cin r' cout' ->
+                  r = r' /\ cout = cout').
+    set (P0 := fun rho e cin r cout =>
+                forall r' cout',
+                  bstep_fuel rho e cin r' cout' ->
+                  r = r' /\ cout = cout').
     intros Hstep.
-    revert r'.
-    induction Hstep using bstep_ind' with (P := P) (P0 := P0); unfold P, P0 in *; intros r' Hstep';
+    revert r' cout'.
+    induction Hstep using bstep_ind' with (P := P) (P0 := P0); unfold P, P0 in *; intros r' cout' Hstep';   
       try now (inv Hstep'; repeat subst_exp; eapply IHHstep; eauto). 
     - inv Hstep'. repeat subst_exp.
       eapply find_tag_nth_deterministic in H1; [| eapply H8 ]. inv H1.
       eapply IHHstep; eauto.
     - inv Hstep'; repeat subst_exp.
-      + eapply bstep_fuel_deterministic in H17; [| clear H17; eauto ]. inv H17; subst. repeat subst_exp.
-        rewrite !(plus_comm cin0) in H10. 
-        eapply plus_inv in H10. subst. eapply IHHstep0; eauto.
-      + eapply bstep_fuel_OOT_monotonic in H17. eapply IHHstep in H17. congruence. 
-    - inv Hstep'; repeat subst_exp; eauto. 
-      eapply bstep_fuel_OOT_determistic in H16; [| eassumption ]. congruence. 
+      + eapply bstep_fuel_deterministic in H18; [| clear H18; eauto ]. destructAll.
+        rewrite !(plus_comm cin0) in H10. eapply plus_inv in H10.
+        subst. edestruct IHHstep0. eapply H19. subst. now eauto.
+      + rewrite plus_comm in H18. eapply bstep_fuel_OOT_monotonic in H18. destructAll.
+        eapply IHHstep in H5. inv H5. congruence. 
+    - inv Hstep'; repeat subst_exp; eauto.       
+      eapply bstep_fuel_OOT_determistic in H17. inv H17. congruence.
+      rewrite plus_comm. eassumption.
     - inv Hstep'. repeat subst_exp; eauto.
     - inv Hstep'; eauto. rewrite plus_comm in H. eapply plus_lt in H. eapply lt_antisym in H.
       contradiction.
     - inv Hstep'; eauto.
       rewrite plus_comm in H. eapply plus_lt in H. eapply lt_antisym in H. contradiction.
-      eapply plus_inv in H. subst. eapply IHHstep. eassumption. 
+      eapply plus_inv in H. subst. edestruct IHHstep. eassumption. subst; eauto.
   Qed.
 
-  Lemma bstep_fuel_deterministic_res rho e r c r' :
-    bstep_fuel rho e r c ->
-    bstep_fuel rho e r' c ->
-    r = r'.
+  Lemma bstep_fuel_deterministic_res rho e cin r r' cout cout' :
+    bstep_fuel rho e cin r cout ->
+    bstep_fuel rho e cin r' cout' ->
+    r = r' /\ cout = cout'.
   Proof.
     intros H1 H2. inv H1; inv H2; eauto.
     rewrite plus_comm in H. eapply plus_lt in H. eapply lt_antisym in H. contradiction.
     rewrite plus_comm in H0. eapply plus_lt in H0. eapply lt_antisym in H0. contradiction.
-    eapply plus_inv in H0. subst. eapply bstep_deterministic_res. eassumption. eassumption.
+    eapply plus_inv in H0. subst. eapply bstep_deterministic_res  in H; [| eassumption ].
+    destructAll. eauto.
   Qed.
   
   
   Definition diverge (rho : env) (e: exp) : Prop :=
-    forall c, bstep_fuel rho e OOT c.
+    forall cin, exists cout, bstep_fuel rho e cin OOT cout.
 
   (** * Interpretation of (certain) evaluation contexts as environments *)
 
@@ -933,7 +1051,6 @@ Section EVAL.
     - simpl; econstructor; eauto.
   Qed.
 
-
   (** * Interpretation of interprable evaluation contexts as environments *)
 
   Fixpoint interprable (C : exp_ctx) : bool :=
@@ -961,121 +1078,138 @@ Section EVAL.
     | Ehole_c => 0
     end.
 
-  Inductive interpret_ctx : exp_ctx -> env -> @res env -> steps -> Prop :=
+  Inductive interpret_ctx : exp_ctx -> env -> fuel -> @res env -> trace -> Prop :=
   | Eproj_c_i :
-      forall rho r t y N Γ C vs v (n : steps),
+      forall rho r t y N Γ C vs v (cin : fuel) (cout : trace),
         M.get Γ rho = Some (Vconstr t vs) ->
         nthN vs N = Some v ->
-        interpret_ctx_fuel C (M.set y v rho) r n ->
-        interpret_ctx (Eproj_c y t N Γ C) rho r n
+        interpret_ctx_fuel C (M.set y v rho) cin r cout ->
+        interpret_ctx (Eproj_c y t N Γ C) rho cin r cout
   | Econstr_c_i :
-      forall rho r x t ys C vs n,
+      forall rho r x t ys C vs (cin : fuel) (cout : trace),
         get_list ys rho = Some vs ->
-        interpret_ctx_fuel C (M.set x (Vconstr t vs) rho) r n ->
-        interpret_ctx (Econstr_c x t ys C) rho r n
+        interpret_ctx_fuel C (M.set x (Vconstr t vs) rho) cin r cout ->
+        interpret_ctx (Econstr_c x t ys C) rho cin r cout
   | Efun_c_i :
-      forall rho r C B n,
-        interpret_ctx_fuel C (def_funs B B rho rho) r n ->
-        interpret_ctx (Efun1_c B C) rho r n
+      forall rho r C B (cin : fuel) (cout : trace),
+        interpret_ctx_fuel C (def_funs B B rho rho) cin r cout ->
+        interpret_ctx (Efun1_c B C) rho cin r cout
   | Eletapp_c_i :
-      forall rho fl rhoc rhoc' f' vs xs e_body c x f t ys v r n1 n2,
+      forall rho fl rhoc rhoc' f' vs xs e_body c x f t ys v r
+             (cin1 cin2 : fuel) (cout1 cout2 : trace),
         rho ! f = Some (Vfun rhoc fl f') ->
         get_list ys rho = Some vs ->
         find_def f' fl = Some (t, xs, e_body) ->
         set_lists xs vs (def_funs fl fl rhoc rhoc) = Some rhoc' ->
-        bstep_fuel rhoc' e_body (Res v) n1 ->
-        interpret_ctx_fuel c (M.set x v rho) r n2 ->
-        interpret_ctx (Eletapp_c x f t ys c) rho r (n1 <+> n2)
+        bstep_fuel rhoc' e_body cin1 (Res v) cout1 ->
+        interpret_ctx_fuel c (M.set x v rho) cin2 r cout2 ->
+        interpret_ctx (Eletapp_c x f t ys c) rho (cin1 <+> cin2) r (cout1 <+> cout2)
   | Eletapp_c_i_OOT :
-      forall rho fl rhoc rhoc' f' vs xs e_body c x f t ys n,
+      forall rho fl rhoc rhoc' f' vs xs e_body c x f t ys (cin : fuel) (cout : trace),
         rho ! f = Some (Vfun rhoc fl f') ->
         get_list ys rho = Some vs ->
         find_def f' fl = Some (t, xs, e_body) ->
         set_lists xs vs (def_funs fl fl rhoc rhoc) = Some rhoc' ->
-        bstep_fuel rhoc' e_body OOT n ->
-        interpret_ctx (Eletapp_c x f t ys c) rho OOT n
-  with interpret_ctx_fuel : exp_ctx -> env -> @res env -> steps -> Prop :=
+        bstep_fuel rhoc' e_body cin OOT cout ->
+        interpret_ctx (Eletapp_c x f t ys c) rho cin OOT cout
+  with interpret_ctx_fuel : exp_ctx -> env -> fuel -> @res env -> trace -> Prop :=
   | ctx_hole:
       forall rho,
-        interpret_ctx_fuel Hole_c rho (Res rho) <0>
+        interpret_ctx_fuel Hole_c rho <0> (Res rho) <0>
   | ctx_OOT :
-      forall c rho n,
-        lt_i (exp_ctx_to_fin c) n (one_ctx c) ->
-        c <> Hole_c ->
-        interpret_ctx_fuel c rho OOT n
+      forall C rho cin,
+        lt cin (one_ctx C) ->
+        C <> Hole_c ->
+        interpret_ctx_fuel C rho cin OOT <0>
   | ctx_step :
-      forall c rho r (n : steps),
-        c <> Hole_c ->
-        interpret_ctx c rho r n  ->
-        interpret_ctx_fuel c rho r (n <+> one_ctx c).
+      forall C rho r (cin : fuel) (cout : trace),
+        C <> Hole_c ->
+        interpret_ctx C rho cin r cout ->
+        interpret_ctx_fuel C rho (cin <+> one_ctx C) r (cout <+> one_ctx C).
   
 
-  Lemma interpret_ctx_bstep_l C e rho v n:
-    bstep_fuel rho (C|[ e ]|) (Res v) n ->
+  Lemma interpret_ctx_bstep_l C e rho v cin cout:
+    bstep_fuel rho (C|[ e ]|) cin (Res v) cout ->
     interprable C = true ->
-    exists rho' n1 n2,
-      (n1 <+> n2) = n /\
-      interpret_ctx_fuel C rho (Res rho') n1 /\
-      bstep_fuel rho' e (Res v) n2.
+    exists rho' cin1 cout1 cin2 cout2,
+      (cin1 <+> cin2) = cin /\
+      (cout1 <+> cout2) = cout /\
+      interpret_ctx_fuel C rho cin1 (Res rho') cout1 /\
+      bstep_fuel rho' e cin2 (Res v) cout2.
   Proof.
-    revert e rho v n; induction C; intros e1 rho v1 c1 Hb Hi; try now inv Hi.
-    - simpl in Hb. exists rho, <0>, c1. split; [| split; eauto ].
-      rewrite plus_zero. reflexivity. econstructor.
+    revert e rho v cin cout; induction C; intros e1 rho v' cin cout Hb Hi; try now inv Hi.
+    - simpl in Hb. eexists rho, (@zero _ fuel _), <0>, cin, cout. split; [| split; eauto ].
+      rewrite plus_zero. reflexivity.
+      rewrite plus_zero. reflexivity.
+      econstructor. econstructor. eassumption. 
     - simpl in Hb, Hi. inv Hb. inv H.
-      edestruct IHC as (rho' & n1 & n2 & Hadd & Hi' & Hstep); [ eassumption | eassumption | ].
-      eexists. exists (n1 <+> one_ctx (Econstr_c v c l C)). eexists. split; [| split; eauto ].
-      2:{ econstructor; eauto. congruence. econstructor; eauto. }
-      rewrite plus_assoc, (plus_comm _ n2), <- plus_assoc. rewrite <- Hadd. reflexivity.
+      edestruct IHC. eassumption. eassumption. destructAll. 
+      do 5 eexists. split; [| split ].
+      3:{ split. econstructor 3. now congruence. econstructor; eauto. eassumption. }
+      rewrite !plus_assoc. rewrite (plus_comm x2). reflexivity.
+      rewrite !plus_assoc. rewrite (plus_comm x3). reflexivity.
     - simpl in Hb, Hi. inv Hb. inv H.
-      edestruct IHC as (rho' & n1 & n2 & Hadd & Hi' & Hstep); [ eassumption | eassumption | ].
-      simpl in Hadd.
-      eexists. exists (n1 <+> one_ctx (Eproj_c v c n v0 C)). eexists. split; [| split; eauto ].
-      2:{ econstructor; eauto. congruence. econstructor; eauto. }
-      rewrite <- Hadd.
-      rewrite plus_assoc, (plus_comm _ n2), <- plus_assoc. simpl. reflexivity.
+      edestruct IHC. eassumption. eassumption. destructAll. 
+      do 5 eexists. split; [| split ].
+      3:{ split. econstructor 3. now congruence. econstructor; eauto. eassumption. }
+      rewrite !plus_assoc. rewrite (plus_comm x2). reflexivity.
+      rewrite !plus_assoc. rewrite (plus_comm x3). reflexivity.
     - simpl in Hb, Hi. inv Hb. inv H.
     - simpl in Hb, Hi. inv Hb. inv H.
-      edestruct IHC as (rho1 & n1 & n2 & Hadd & Hi' & Hstep); [ eassumption | eassumption | ].
-      eexists. exists (cin1 <+> n1 <+> one_ctx (Eletapp_c v v0 f l C))%nat.
-      eexists. split; [| split; eauto ].
-      2:{ econstructor; eauto. congruence. econstructor; eauto. }
-      rewrite <- Hadd.
-      rewrite plus_assoc, (plus_comm _ n2), <- !plus_assoc. simpl. reflexivity.      
+      edestruct IHC. eassumption. eassumption. destructAll. repeat subst_exp. 
+      do 5 eexists. split; [| split ]. 
+      3:{ split; [| eassumption ].
+          econstructor 3. now congruence. econstructor; eauto. }
+      rewrite !plus_assoc. rewrite (plus_comm x2). reflexivity.
+      rewrite !plus_assoc. rewrite (plus_comm x3). reflexivity.
     - simpl in Hb, Hi. inv Hb. inv H.
-      edestruct IHC as (rho' & n1 & n2 & Hadd & Hi' & Hstep); [ eassumption | eassumption | ].
-      simpl in Hadd.
-      eexists. exists (n1 <+> one_ctx (Efun1_c f C)). eexists. split; [| split; eauto ].
-      2:{ econstructor; eauto. congruence. econstructor; eauto. }
-      simpl in *.
-      rewrite <- Hadd.
-      rewrite plus_assoc, (plus_comm _ n2), <- plus_assoc. simpl. reflexivity.
+      edestruct IHC. eassumption. eassumption. destructAll. 
+      do 5 eexists. split; [| split ].
+      3:{ split. econstructor 3. now congruence. econstructor; eauto. eassumption. }
+      rewrite !plus_assoc. rewrite (plus_comm x2). reflexivity.
+      rewrite !plus_assoc. rewrite (plus_comm x3). reflexivity.
   Qed.
 
-  Lemma interpret_ctx_bstep_r C e rho rho' r n1 n2:
-    interpret_ctx_fuel C rho (Res rho') n1 ->
-    bstep_fuel rho' e r n2 ->
-    bstep_fuel rho (C|[ e ]|) r (n1 <+> n2).
+  Lemma interpret_ctx_bstep_r C e rho rho' r cin1 cin2 cout1 cout2 :
+    interpret_ctx_fuel C rho cin1 (Res rho') cout1 ->
+    bstep_fuel rho' e cin2 r cout2 ->
+    bstep_fuel rho (C|[ e ]|) (cin1 <+> cin2) r (cout1 <+> cout2).
   Proof.
-    revert e rho rho' r n1 n2; induction C; intros e1 rho rho' r n1 n2 Hi Hs1; (try now inv Hi);
-      try (now (inv Hi; inv H0;
-                rewrite plus_assoc, (plus_comm (one_ctx _)), <- plus_assoc;
-                econstructor; econstructor; eauto)).
-    - inv Hi. simpl. rewrite plus_zero. eassumption. simpl.
-      inv H0.
-    - inv Hi. inv H0. simpl in *.
-      rewrite plus_assoc, (plus_comm (one_ctx _)), <- plus_assoc.
-      econstructor. rewrite plus_assoc. econstructor; eauto.       
+    revert e rho rho' r cin1 cin2 cout1 cout2; induction C;
+      intros e1 rho rho' r cin1 cin2 cout1 cout2 Hi Hs1; (try now inv Hi);
+              try (now (inv Hi; inv H0;
+                        rewrite !plus_assoc, !(plus_comm (one_ctx _)), <- !plus_assoc;
+                        econstructor; econstructor; eauto)).
+    - inv Hi. simpl. rewrite !plus_zero. eassumption. inv H0.
+    - inv Hi. inv H0. simpl.
+      rewrite !plus_assoc, !(plus_comm (one_ctx _)), <- !plus_assoc.
+      econstructor. rewrite !plus_assoc. econstructor; eauto.       
   Qed.
 
-  Lemma interpret_ctx_OOT_bstep C e rho n:
-    interpret_ctx_fuel C rho OOT n ->
-    bstep_fuel rho (C|[ e ]|) OOT n.
+  Lemma interpret_ctx_OOT_bstep C e rho cin cout:
+    interpret_ctx_fuel C rho cin OOT cout ->
+    exists cout' c, bstep_fuel rho (C|[ e ]|) cin OOT cout' /\ cout = (c <+> cout').
   Proof.
-    revert e rho n; induction C; intros e1 rho n1 Hi; (try now inv Hi);
-      try now (inv Hi; simpl in *;
-               [ econstructor 1; eassumption |
-                 inv H0; econstructor 2; econstructor; eauto
-              ]).
+    revert e rho cin cout; induction C; intros e1 rho cin cout' Hi; (try now inv Hi);    
+      try now (inv Hi; [ do 2 eexists; split; [ econstructor 1; eauto | rewrite plus_zero; reflexivity ] 
+                       | inv H0; edestruct IHC; eauto; destructAll; do 2 eexists; split;
+                       [ econstructor 2; eauto; econstructor; eauto | rewrite plus_assoc; reflexivity ] ]).
+    - inv Hi; [ do 2 eexists; split; [ econstructor 1; eauto | rewrite plus_zero; reflexivity ] 
+              | inv H0 ].
+    - inv Hi.
+      + do 2 eexists; split; [ econstructor 1; eauto | rewrite plus_zero; reflexivity ].
+      + inv H0.
+        * edestruct IHC; eauto; destructAll; do 2 eexists; split.
+          econstructor 2; eauto; econstructor; eauto.
+          rewrite <- plus_assoc. rewrite (plus_comm cout1).
+          do 2 rewrite plus_assoc.
+          rewrite (plus_assoc cout1 x (one _)). reflexivity.
+        * do 2 eexists. split. econstructor 2; eauto. econstructor; eauto.
+          rewrite plus_zero. reflexivity.
+    - inv Hi; [ do 2 eexists; split; [ econstructor 1; eauto | rewrite plus_zero; reflexivity ] 
+              | inv H0; edestruct IHC; eauto ].
+    - inv Hi; [ do 2 eexists; split; [ econstructor 1; eauto | rewrite plus_zero; reflexivity ] 
+              | inv H0; edestruct IHC; eauto ].
   Qed.
 
   Lemma interprable_comp_f_l C1 C2:
@@ -1106,51 +1240,13 @@ Section EVAL.
   Qed.
 
 
-  (* 
-  Lemma eval_ctx_app_OOT_Ehalt rho C e n x :
-    bstep_fuel rho (C |[ Ehalt x ]|) OOT n ->
+  Lemma eval_ctx_app_OOT_Eprim rho C x p xs e1 e2 cin cout :
+    bstep_fuel rho (C |[ Eprim x p xs e1 ]|) cin OOT cout ->
     interprable C = true ->
-    bstep_fuel rho (C |[ e ]|) OOT n.
-  Proof.
-    revert rho e n.
-    induction C; intros rho e1 cin Hs Hi; eauto;
-      try congruence;
-      try now (simpl in *; inv Hs; 
-               [ econstructor; eassumption |
-                 inv H; unfold one; simpl; constructor 2; econstructor; eauto ]).
-    
-    - simpl in *. inv Hs. econstructor. eapply lt_zero_one in H. subst. eapply zero_one_lt_i.
-      inv H.
-
-      Unshelve. exact 0%nat.
-  Qed.
-  
-  Lemma eval_ctx_app_OOT_Eapp rho C e n x f t xs :
-    bstep_fuel rho (C |[ Eapp f t xs ]|) OOT n ->
-    interprable C = true ->
-    bstep_fuel rho (C |[ Eletapp x f t xs e ]|) OOT n.
-  Proof.
-    revert rho e n.
-    induction C; intros rho e1 cin Hs Hi; eauto;
-      try congruence;
-      try now (inv Hs; 
-               [ econstructor; eassumption |
-                 inv H; unfold one; simpl; constructor 2; econstructor; eauto ]).
-
-    simpl in *. inv Hs. econstructor. eapply lt_zero_one in H. subst. eapply zero_one_lt_i.
-    inv H. erewrite <- one_letapp. econstructor 2. econstructor; eauto.    
-    
-    Unshelve. exact 0%nat.
-  Qed.
-
-  
-  Lemma eval_ctx_app_OOT_Eprim rho C x p xs e1 e2 n :
-    bstep_fuel rho (C |[ Eprim x p xs e1 ]|) OOT n ->
-    interprable C = true ->
-    bstep_fuel rho (C |[ Eprim x p xs e2 ]|) OOT n.
+    bstep_fuel rho (C |[ Eprim x p xs e2 ]|) cin OOT cout.
   Proof.       
-    revert rho n.
-    induction C; intros rho cin Hs Hi; eauto;
+    revert rho cin cout.
+    induction C; intros rho cin cout Hs Hi; eauto;
       try congruence;
       try now (inv Hs; 
                [ econstructor; eassumption |
@@ -1159,30 +1255,48 @@ Section EVAL.
 
     Unshelve. exact 0%nat.
   Qed.
-  *)
   
-  Lemma bstep_cost_deterministic e rho v1 v2 c1 c2 :
-    bstep_cost rho e v1 c1 ->
-    bstep_cost rho e v2 c2 ->
-    v1 = v2 /\ c1 = c2.
-  Proof.
-    intros Heval1 Heval2.
-    revert v2 c2 Heval2; induction Heval1; intros v2 c2 Heval2;
-      inv Heval2; repeat subst_exp; eauto;
-        try now edestruct IHHeval1 as [Heq1 Heq2]; eauto.
-    + eapply find_tag_nth_deterministic in H7; [| clear H7; eauto ]; inv H7.
-      eapply IHHeval1 in H10. inv H10. split; congruence.
-    + eapply IHHeval1_1 in H15. inv H15.
-      eapply IHHeval1_2 in H16. inv H16.
-      split; congruence.
-  Qed.
 
-  Lemma interpret_ctx_eq_env_P S C rho rho' n :
-    interpret_ctx_fuel C rho (Res rho') n ->
+  Lemma eval_ctx_app_OOT_Eapp rho C e cin cout x f t xs :
+    bstep_fuel rho (C |[ Eapp f t xs ]|) cin OOT cout ->
+    interprable C = true ->
+    bstep_fuel rho (C |[ Eletapp x f t xs e ]|) cin OOT cout.
+  Proof.
+    revert rho e cin cout.
+    induction C; intros rho e1 cin cout Hs Hi; eauto;
+      try congruence;
+      try now (inv Hs; 
+               [ econstructor; eassumption |
+                 inv H; unfold one; simpl; constructor 2; econstructor; eauto ]).
+    
+    Unshelve. exact 0%nat.
+  Qed.
+      
+  Lemma eval_ctx_app_Ehalt_div rho C e cin cout x :
+    bstep_fuel rho (C |[ Ehalt x ]|) cin OOT cout ->
+    interprable C = true ->
+    bstep_fuel rho (C |[ e ]|) cin OOT cout.
+  Proof.
+    revert rho e cin cout.
+    induction C; intros rho e1 cin cout Hs Hi; eauto;
+      try congruence;
+      try now (inv Hs; 
+               [ econstructor; eassumption |
+                 inv H; unfold one; simpl; constructor 2; econstructor; eauto ]).
+    simpl in *. inv Hs.
+    2:{ inv H. }
+    econstructor. unfold one. erewrite one_eq. eassumption.
+    
+    Unshelve. exact 0%nat.
+  Qed.
+  
+    
+  Lemma interpret_ctx_eq_env_P S C rho rho' cin cout :
+    interpret_ctx_fuel C rho cin (Res rho') cout ->
     Disjoint _ (bound_var_ctx C) S ->
     eq_env_P S rho rho'.
   Proof.
-    revert rho rho' n; induction C; intros rho rho' cost Hin Hd; inv Hin.
+    revert rho rho' cin cout; induction C; intros rho rho' cin cout Hin Hd; inv Hin.
     - eapply eq_env_P_refl.
     - inv H0.
     - inv H0. rewrite bound_var_Econstr_c in *.
@@ -1210,30 +1324,30 @@ Section EVAL.
   Scheme interpret_ctx_ind' := Minimality for interpret_ctx Sort Prop
     with interpret_ctx_fuel_ind' := Minimality for interpret_ctx_fuel Sort Prop.
 
-  Lemma interpret_ctx_deterministic_aux rho C r v c r' v' c' :
-    interpret_ctx C rho r c ->
-    interpret_ctx C rho r' c' ->
+  Lemma interpret_ctx_deterministic_aux rho C r v cin cout r' v' cin' cout' :
+    interpret_ctx C rho cin r cout ->
+    interpret_ctx C rho cin' r' cout' ->
     r = Res v -> r' = Res v' ->
-    v = v' /\ c = c'.
+    v = v' /\ cin = cin' /\ cout = cout'.
   Proof.
-    set (R := fun C rho r c =>
-                forall v r' v' c',
-                  interpret_ctx C rho r' c' ->
+    set (R := fun C rho cin r cout =>
+                forall v r' v' cin' cout',
+                  interpret_ctx C rho cin' r' cout' ->
                   r = Res v -> r' = Res v' ->
-                  v = v' /\ c = c').
-    set (R0 := fun C rho r c =>
-                 forall v r' v' c',
-                   interpret_ctx_fuel C rho r' c' ->
-                   r = Res v -> r' = Res v' ->
-                   v = v' /\ c = c').
+                  v = v' /\ cin = cin' /\ cout = cout').
+    set (R0 := fun C rho cin r cout =>
+                forall v r' v' cin' cout',
+                  interpret_ctx_fuel C rho cin' r' cout' ->
+                  r = Res v -> r' = Res v' ->
+                  v = v' /\ cin = cin' /\ cout = cout').
     intros Hint.
-    revert v r' v' c'.
+    revert v r' v' cin' cout'.
     induction Hint using interpret_ctx_ind' with (P := R) (P0 := R0); unfold R, R0 in *;
-      intros v1 r2 v2 c2 Hint2 Heq1 Heq2; subst;
+      intros v1 r2 v2 cin' cout' Hint2 Heq1 Heq2; subst;
         (try now inv Hint2; repeat subst_exp; eapply IHHint; [ eassumption | reflexivity | reflexivity ]).
     - inv Hint2. repeat subst_exp.
-      eapply bstep_fuel_deterministic in H17; [| clear H17; eassumption ]. destructAll.
-      eapply IHHint in H18; eauto. destructAll. split; eauto.
+      eapply bstep_fuel_deterministic in H18; [| clear H18; eassumption ]. destructAll.
+      eapply IHHint in H19; eauto. destructAll. split; eauto.
     - inv Heq1.
     - inv Hint2. inv Heq1; eauto. inv H0.
     - inv Heq1.
@@ -1241,78 +1355,80 @@ Section EVAL.
       eapply IHHint in H1; eauto. destructAll. split; eauto.
   Qed.
 
-  Lemma interpret_ctx_fuel_deterministic C rho v c v' c' :
-    interpret_ctx_fuel C rho (Res v) c ->
-    interpret_ctx_fuel C rho (Res v') c' ->
-    v = v' /\ c = c'.
+  Lemma interpret_ctx_fuel_deterministic C rho v v' cin cin' cout cout' :
+    interpret_ctx_fuel C rho cin (Res v) cout ->
+    interpret_ctx_fuel C rho cin' (Res v') cout' ->
+    v = v' /\ cin = cin' /\ cout = cout'.
   Proof.
     intros H1 H2; inv H1; inv H2; eauto.
     - congruence.
     - congruence.
     - eapply interpret_ctx_deterministic_aux in H0; [ | clear H0; eassumption | reflexivity | reflexivity ].
-      inv H0. eauto.
+      destructAll. eauto.
   Qed.
 
-  Lemma interpret_ctx_deterministic C rho v c v' c' :
-    interpret_ctx C rho (Res v) c ->
-    interpret_ctx C rho (Res v') c' ->
-    v = v' /\ c = c'.
+  Lemma interpret_ctx_deterministic C rho v v' cin cin' cout cout' :
+    interpret_ctx C rho cin (Res v) cout ->
+    interpret_ctx C rho cin' (Res v') cout' ->
+    v = v' /\ cin = cin' /\ cout = cout'.
   Proof.
     intros H1 H2.
     eapply interpret_ctx_deterministic_aux; eauto.
   Qed.
 
-  Lemma bstep_fuel_ctx_OOT rho C e c :
-    bstep_fuel rho (C |[ e ]|) OOT c ->
+  Lemma bstep_fuel_ctx_OOT rho C e cin cout :
+    bstep_fuel rho (C |[ e ]|) cin OOT cout ->
     interprable C = true ->
-    interpret_ctx_fuel C rho OOT c \/
-    exists rho' c1 c2,
-      interpret_ctx_fuel C rho (Res rho') c1 /\
-      bstep_fuel rho' e OOT c2 /\
-      c = (c1 <+> c2).
+    interpret_ctx_fuel C rho cin OOT cout \/
+    exists rho' cin1 cin2 cout1 cout2,
+      interpret_ctx_fuel C rho cin1 (Res rho') cout1 /\
+      bstep_fuel rho' e cin2 OOT cout2 /\
+      cin = (cin1 <+> cin2) /\ cout = (cout1 <+> cout2).
   Proof.
-    revert rho e c. induction C; intros rho e1 c1 Hstep Hi; (try now inv Hi); simpl in Hi.
-    - simpl in Hstep. right. eexists. exists <0>. eexists.
-      split. econstructor. split; eauto. rewrite plus_zero; eauto.
-    - inv Hstep.
-      + left. econstructor; [| congruence ]. eassumption.
-      + inv H. eapply IHC in H9; eauto. inv H9.
-        * left. eapply ctx_step; [ congruence | econstructor; eauto ].
-        * destructAll. right. do 3 eexists.
-          split; [| split ]; [| eassumption |]. econstructor. congruence. econstructor; eauto.
-          rewrite (plus_assoc _ _ x1), (plus_comm (one_ctx _) x1), <- plus_assoc. reflexivity.
+    revert rho e cin cout. induction C; intros rho e1 cin cout Hstep Hi; (try now inv Hi); simpl in Hi.
+    - simpl in Hstep. right. do 5 eexists. split. econstructor. split. eassumption.
+      rewrite !plus_zero; eauto.
     - inv Hstep.
       + left. econstructor; [| congruence ]. eassumption.
       + inv H. eapply IHC in H10; eauto. inv H10.
         * left. eapply ctx_step; [ congruence | econstructor; eauto ].
-        * destructAll. right. do 3 eexists.
+        * destructAll. right. do 5 eexists.
           split; [| split ]; [| eassumption |]. econstructor. congruence. econstructor; eauto.
-          rewrite (plus_assoc _ _ x1), (plus_comm (one_ctx _) x1), <- plus_assoc. reflexivity.          
+          rewrite (plus_assoc _ _ x1), (plus_comm (one_ctx _) x1), <- plus_assoc.
+          rewrite (plus_assoc _ _ x3), (plus_comm (one_ctx _) x3), <- plus_assoc. eauto.
+    - inv Hstep.
+      + left. econstructor; [| congruence ]. eassumption.
+      + inv H. eapply IHC in H11; eauto. inv H11.
+        * left. eapply ctx_step; [ congruence | econstructor; eauto ].
+        * destructAll. right. do 5 eexists.
+          split; [| split ]; [| eassumption |]. econstructor. congruence. econstructor; eauto.
+          rewrite (plus_assoc _ _ x1), (plus_comm (one_ctx _) x1), <- plus_assoc.
+          rewrite (plus_assoc _ _ x3), (plus_comm (one_ctx _) x3), <- plus_assoc. eauto.
     - inv Hstep.
       + left. econstructor; [| congruence ]. eassumption.
       + inv H.
     - inv Hstep.
       + left. econstructor; [| congruence ]. eassumption.
       + inv H.
-        * eapply IHC in H13. inv H13.
+        * eapply IHC in H14. inv H14.
           -- left. eapply ctx_step. congruence. econstructor; eauto.
-          -- destructAll. right. do 3 eexists.
+          -- destructAll. right. do 5 eexists.
              split; [| split ].
-             econstructor. congruence. now econstructor; eauto. eassumption.
-             rewrite !plus_assoc. f_equal. f_equal. rewrite plus_comm. f_equal.
+             econstructor. congruence. now econstructor; eauto. eassumption. split. 
+             rewrite (plus_assoc _ _ x1), (plus_comm (one_ctx _) x1), <- !plus_assoc. reflexivity.
+             rewrite (plus_assoc _ _ x3), (plus_comm (one_ctx _) x3), <- !plus_assoc. reflexivity.
           -- eassumption.
         * left. eapply ctx_step. congruence. econstructor; eauto.
     - inv Hstep.
       + left. econstructor; [| congruence ]. eassumption.
-      + inv H. eapply IHC in H5; eauto. inv H5.
+      + inv H. eapply IHC in H6; eauto. inv H6.
         * left. unfold one_ctx. eapply ctx_step; [ congruence | econstructor; eauto ].
-        * destructAll. right. do 3 eexists.
+        * destructAll. right. do 5 eexists.
           split; [| split ]; [| eassumption |]. econstructor. congruence. econstructor; eauto.
-          rewrite (plus_assoc _ _ x1), (plus_comm (one_ctx _) x1), <- plus_assoc. reflexivity.
+          rewrite (plus_assoc _ _ x1), (plus_comm (one_ctx _) x1), <- plus_assoc.
+          rewrite (plus_assoc _ _ x3), (plus_comm (one_ctx _) x3), <- plus_assoc. eauto.
   Qed.
-
-  
-  
+    
   (** Small step semantics -- Relational definition *)
   (* Zoe : How to write small step for letapp? *)
   Inductive step: state -> state -> Prop :=
